lecture14-dafny-code/lecture14/methods-with-specs.dfy
@@ -1,0 +1,37 @@
+method maxMinMethod(i : int, j : int) returns (mx : int, mn:int)
+  /* parens required around returns, even if there's only one */
+  ensures mx == max(i,j)
+  // and what else?
+{
+    if i < j { mx := j; mn := i; }
+    else { mx := i; mn := j; }
+}
+
+function max(i : int, j : int) : int 
+{
+    if i < j then j else i
+}
+
+function min(i:int, j:int) : int
+{ 
+    if i < j then i else j
+}
+
+method clamp(x: int, lo: int, hi: int) returns (r: int)
+  ensures true // <--- FIX ME
+{
+  if x < lo { return lo; }
+  if x > hi { return hi; }
+  return x;  // could be r := x;
+}
+
+method divmod(m:nat, n:nat) returns (ok:bool,q:nat,r:nat)
+  ensures true // <--- FIX ME
+{
+    // could also write return false,0,0;
+    if n == 0 { 
+        ok,q,r := false,0,0; 
+        return; 
+    }
+    ok,q,r := true, m/n, m%n;
+}
