lecture14-dafny-code/lecture14/methodspec-opacity.dfy
@@ -1,0 +1,30 @@
+function max(i:int, j:int) : int
+{ if i < j then j else i}
+
+function exceed(i:int, j :int) : int
+{ max(i,j) + 1}
+
+lemma exceed_correct(i:int, j:int)
+  ensures exceed(i,j) > i
+  ensures exceed(i,j) > j 
+{}
+
+// In the Land of Methods things are not quite so rosy
+
+method maxMethod(i:int, j:int) returns (mx:int)
+{
+    if i < j { mx := j; } else { mx := i; }
+}
+
+// this doesn't work
+lemma maxMethod_lemma(i:int, j:int)
+//  ensures maxMethod(i,j) == max(i,j)
+{}
+
+method exceedMethod(i:int, j:int) returns (exceeder:int)
+  //ensures exceeder > i 
+  //ensures exceeder > j
+{
+    var mx := maxMethod(i,j);
+    exceeder := mx + 1;
+}
