lecture14-dafny-code/lecture14/simple-methods.dfy
@@ -1,0 +1,15 @@
+/* What *must* we assign to?  What *mustn't* we assign to? */
+method maxMinMethod(i : int, j : int) returns (mx : int, mn:int)
+  /* parens required around returns, even if there's only one */
+{
+    if i < j { mx := j; mn := i; }
+    else { mx := i; mn := j ;}
+    // i := 3; 不能给输入的变量赋值
+}
+
+method Main()
+{
+    // dafny is fussy here; can't put parens around x,n
+    var x,n := maxMinMethod(10,3);
+    print "Min is ", n, "; max is ", x, "\n";
+}
